src/burrow/live_rec.v
@@ -1,0 +1,208 @@
+From iris.algebra Require Export cmra.
+From iris.algebra Require Import proofmode_classes.
+From iris.prelude Require Import options.
+Require Import cpdt.CpdtTactics.
+
+From stdpp Require Import gmap.
+From stdpp Require Import mapset.
+From stdpp Require Import sets.
+From stdpp Require Import list.
+Require Import Burrow.trees.
+Require Import Burrow.indexing.
+Require Import Burrow.tactics.
+Require Import Burrow.locations.
+Require Import Burrow.resource_proofs.
+Require Import Burrow.exchanges.
+Require Import Burrow.assoc_comm.
+Require Import coq_tricks.Deex.
+
+Section LiveRec.
+
+Context {M} `{!EqDecision M} `{!TPCM M}.
+Context {RI} `{!EqDecision RI, !Countable RI, !RefinementIndex M RI}.
+
+Fixpoint live_rec (loc: Loc RI) (m: M) :=
+      match loc with
+    | BaseLoc _ _ => live loc m
+    | ExtLoc _ _ _ => live loc m
+    | CrossLoc l r =>
+          (live_rec l (rel M M (refinement_of (left_ri RI)) m)) ⋅
+          (live_rec r (rel M M (refinement_of (right_ri RI)) m))
+  end.
+
+Lemma live_rec_eq (l r : Loc RI) (m1 m2 : M)
+    : live_rec (CrossLoc l r) (pair_up RI m1 m2) = live_rec l m1 ⋅ live_rec r m2.
+Proof.
+  cbn [live_rec]. f_equal.
+  - f_equal. apply refinement_of_left_pair_up.
+  - f_equal. apply refinement_of_right_pair_up.
+Qed.
+
+Lemma update_a (a a' b c : State M RI)
+  (u: ∀ p , ✓(a ⋅ p) → ✓(a' ⋅ p))
+  : ✓(a ⋅ b ⋅ c) -> ✓(a' ⋅ b ⋅ c).
+Proof.
+   setoid_replace (a ⋅ b ⋅ c) with (a ⋅ (b ⋅ c)) by solve_assoc_comm.
+   setoid_replace (a' ⋅ b ⋅ c) with (a' ⋅ (b ⋅ c)) by solve_assoc_comm.
+   apply u.
+Qed.
+  
+Lemma update_b (a b b' c : State M RI)
+  (u: ∀ p , ✓(b ⋅ p) → ✓(b' ⋅ p))
+  : ✓(a ⋅ b ⋅ c) -> ✓(a ⋅ b' ⋅ c).
+Proof.
+   setoid_replace (a ⋅ b ⋅ c) with (b ⋅ (a ⋅ c)) by solve_assoc_comm.
+   setoid_replace (a ⋅ b' ⋅ c) with (b' ⋅ (a ⋅ c)) by solve_assoc_comm.
+   apply u.
+Qed.
+
+Lemma pair_up_unit_unit
+    : (pair_up RI (unit: M) unit) = unit.
+Proof.
+  assert (pair_up RI (unit: M) (unit: M) =
+      pair_up RI (rel M M (refinement_of (left_ri RI)) unit)
+                 (rel M M (refinement_of (right_ri RI)) unit)) as X.
+  { rewrite rel_unit. rewrite rel_unit. trivial. }
+  rewrite X.
+  rewrite <- self_eq_pair.
+  trivial.
+Qed.
+
+Lemma unit_unit_pair_is_unit (loc1 loc2: Loc RI)
+  : live (CrossLoc loc1 loc2) (pair_up RI (unit: M) unit) ≡ (state_unit : State M RI).
+Proof.
+  rewrite pair_up_unit_unit. apply live_unit.
+Qed.
+
+Lemma op_state_unit_left x : state_unit ⋅ x ≡ x.
+Proof. setoid_rewrite state_comm. apply op_state_unit. Qed.
+
+Lemma live_split1 (loc1 loc2 : Loc RI) (m1 m2 : M) p
+  (Q : ✓ (live (CrossLoc loc1 loc2) (pair_up RI m1 m2) ⋅ p))
+  : ✓ (live loc1 m1 ⋅ live loc2 m2 ⋅ p).
+Proof.
+  assert (live loc1 m1 ≡ live loc1 m1 ⋅ live (CrossLoc loc1 loc2) (pair_up RI unit unit)) as X.
+  { setoid_rewrite unit_unit_pair_is_unit. setoid_rewrite op_state_unit. trivial. }
+  setoid_rewrite X.
+  apply update_a with (a :=
+    live loc1 unit ⋅ live (CrossLoc loc1 loc2) (pair_up RI m1 unit)
+  ).
+  { intro. apply swap_cross_left_valid. }
+  setoid_rewrite live_unit.
+  setoid_rewrite op_state_unit_left.
+  setoid_replace (live (CrossLoc loc1 loc2) (pair_up RI m1 unit) ⋅ live loc2 m2) with
+                 (live loc2 m2 ⋅ live (CrossLoc loc1 loc2) (pair_up RI m1 unit))
+                 by (apply state_comm).
+  apply swap_cross_right_valid. 
+  setoid_rewrite live_unit.
+  setoid_rewrite op_state_unit_left.
+  trivial.
+Qed.
+
+Lemma live_join1 (loc1 loc2 : Loc RI) (m1 m2 : M) p
+  (Q: ✓ (live loc1 m1 ⋅ live loc2 m2 ⋅ p))
+  : ✓ (live (CrossLoc loc1 loc2) (pair_up RI m1 m2) ⋅ p).
+Proof.
+  setoid_replace (live (CrossLoc loc1 loc2) (pair_up RI m1 m2))
+      with (live loc1 unit ⋅ live (CrossLoc loc1 loc2) (pair_up RI m1 m2))
+      by (setoid_rewrite live_unit; setoid_rewrite op_state_unit_left; trivial).
+  apply swap_cross_left_valid.
+  setoid_replace (live (CrossLoc loc1 loc2) (pair_up RI unit m2))
+      with (live loc2 unit ⋅ live (CrossLoc loc1 loc2) (pair_up RI unit m2))
+      by (setoid_rewrite live_unit; setoid_rewrite op_state_unit_left; trivial).
+  apply update_b with (b :=
+    live loc2 m2 ⋅ live (CrossLoc loc1 loc2) (pair_up RI unit unit)
+  ).
+  { intro. apply swap_cross_right_valid. }
+  setoid_rewrite unit_unit_pair_is_unit.
+  setoid_rewrite op_state_unit.
+  trivial.
+Qed.
+
+Lemma live_split (loc1 loc2 : Loc RI) (m : M) p
+  (Q: ✓ (live (CrossLoc loc1 loc2) m ⋅ p))
+  : ✓ (live loc1 (rel M M (refinement_of (left_ri RI)) m)
+     ⋅ live loc2 (rel M M (refinement_of (right_ri RI)) m) ⋅ p).
+Proof.
+  rewrite (self_eq_pair m) in Q. apply live_split1. trivial.
+Qed.
+
+Lemma live_join (loc1 loc2 : Loc RI) (m : M) p
+  (Q: ✓ (live loc1 (rel M M (refinement_of (left_ri RI)) m)
+     ⋅ live loc2 (rel M M (refinement_of (right_ri RI)) m) ⋅ p))
+  : ✓ (live (CrossLoc loc1 loc2) m ⋅ p).
+Proof.
+  rewrite (self_eq_pair m). apply live_join1. trivial.
+Qed.
+
+Lemma live_to_live_rec (loc: Loc RI) (m: M) p
+   : ✓(live loc m ⋅ p) -> ✓(live_rec loc m ⋅ p).
+Proof.
+  generalize p. clear p. generalize m. clear m. induction loc.
+  - trivial.
+  - trivial.
+  - cbn [live_rec]. intros.
+      apply update_a with (a := live loc1 (rel M M (refinement_of (left_ri RI)) m)).
+      { intro. apply IHloc1. }
+      apply update_b with (b := live loc2 (rel M M (refinement_of (right_ri RI)) m)).
+      { intro. apply IHloc2. }
+      apply live_split. trivial.
+Qed.
+
+Lemma live_rec_to_live (loc: Loc RI) (m: M) p
+   : ✓(live_rec loc m ⋅ p) -> ✓(live loc m ⋅ p).
+Proof.
+  generalize p. clear p. generalize m. clear m. induction loc.
+  - trivial.
+  - trivial.
+  - cbn [live_rec]. intros.
+      apply live_join.
+      apply update_a with (a := live_rec loc1 (rel M M (refinement_of (left_ri RI)) m)).
+      { intro. apply IHloc1. }
+      apply update_b with (b := live_rec loc2 (rel M M (refinement_of (right_ri RI)) m)).
+      { intro. apply IHloc2. }
+      trivial.
+Qed.
+
+Lemma ref_left_dot (m1 m2: M)
+  : rel M M (refinement_of (left_ri RI)) (dot m1 m2) =
+  dot (rel M M (refinement_of (left_ri RI)) m1) (rel M M (refinement_of (left_ri RI)) m2).
+Proof.
+  rewrite (self_eq_pair m1).
+  rewrite (self_eq_pair m2).
+  rewrite dot_pair_up.
+  rewrite <- (self_eq_pair m1).
+  rewrite <- (self_eq_pair m2).
+  rewrite refinement_of_left_pair_up.
+  trivial.
+Qed.
+
+Lemma ref_right_dot (m1 m2: M)
+  : rel M M (refinement_of (right_ri RI)) (dot m1 m2) =
+  dot (rel M M (refinement_of (right_ri RI)) m1) (rel M M (refinement_of (right_ri RI)) m2).
+Proof.
+  rewrite (self_eq_pair m1).
+  rewrite (self_eq_pair m2).
+  rewrite dot_pair_up.
+  rewrite <- (self_eq_pair m1).
+  rewrite <- (self_eq_pair m2).
+  rewrite refinement_of_right_pair_up.
+  trivial.
+Qed.
+
+Lemma live_rec_dot_live_rec
+    (gamma: Loc RI) (m1 m2: M)
+    : live_rec gamma m1 ⋅ live_rec gamma m2 ≡ live_rec gamma (dot m1 m2).
+Proof.
+  generalize m1. clear m1. generalize m2. clear m2. induction gamma.
+  - intros. unfold live_rec. apply live_dot_live.
+  - intros. unfold live_rec. apply live_dot_live.
+  - intros. cbn [live_rec].
+      rewrite ref_left_dot.
+      rewrite ref_right_dot.
+      setoid_rewrite <- IHgamma1.
+      setoid_rewrite <- IHgamma2.
+      solve_assoc_comm.
+Qed.
+
+End LiveRec.
